@prefix : <https://purl.org/wodt/> .
@prefix dc: <http://purl.org/dc/elements/1.1/> .
@prefix owl: <http://www.w3.org/2002/07/owl#> .
@prefix rdf: <http://www.w3.org/1999/02/22-rdf-syntax-ns#> .
@prefix xml: <http://www.w3.org/XML/1998/namespace> .
@prefix xsd: <http://www.w3.org/2001/XMLSchema#> .
@prefix foaf: <http://xmlns.com/foaf/0.1/> .
@prefix rdfs: <http://www.w3.org/2000/01/rdf-schema#> .
@prefix time: <http://www.w3.org/2006/time#> .
@prefix vann: <http://purl.org/vocab/vann/> .
@prefix dcterms: <http://purl.org/dc/terms/> .
@base <https://purl.org/wodt/> .

<https://purl.org/wodt/> rdf:type owl:Ontology ;
                          dc:rights "This ontology is licensed under Apache 2.0" ;
                          dcterms:creator [ rdf:type foaf:Person ;
                                            foaf:name "Andrea" ;
                                            foaf:surname "Giulianelli"
                                          ] ;
                          dcterms:description "The WoDT vocabulary supports the Hypermedia-based WoDT proposal"@en ;
                          dcterms:license <https://www.apache.org/licenses/LICENSE-2.0> ;
                          dcterms:title "WoDT vocabulary" ;
                          vann:preferredNamespacePrefix "wodt" ;
                          rdfs:label "WoDT vocabulary"@en ;
                          owl:versionInfo "1.0.0" .

#################################################################
#    Annotation properties
#################################################################

###  http://purl.org/dc/elements/1.1/rights
dc:rights rdf:type owl:AnnotationProperty .


###  http://purl.org/dc/terms/creator
dcterms:creator rdf:type owl:AnnotationProperty .


###  http://purl.org/dc/terms/description
dcterms:description rdf:type owl:AnnotationProperty .


###  http://purl.org/dc/terms/license
dcterms:license rdf:type owl:AnnotationProperty .


###  http://purl.org/dc/terms/title
dcterms:title rdf:type owl:AnnotationProperty .


###  http://purl.org/vocab/vann/preferredNamespacePrefix
vann:preferredNamespacePrefix rdf:type owl:AnnotationProperty .


###  http://xmlns.com/foaf/0.1/name
foaf:name rdf:type owl:AnnotationProperty .


###  http://xmlns.com/foaf/0.1/surname
foaf:surname rdf:type owl:AnnotationProperty .


###  https://purl.org/wodt/domainTag
:domainTag rdf:type owl:AnnotationProperty ;
           rdfs:comment """The domain tag annotation property allows to annotate the Digital Twin model with domain-oriented semantic annotations. It is purposely designed with an open range to include the possibility to use every type of semantic information available -- classes, individuals, and so on.

A particular use case is the association of domain-related information to the properties, actions, and events of the WoT Thing Description used to implement the Digital Twin Description -- that at the moment only include the possibility to associate classes (via @type)."""@en ;
           rdfs:isDefinedBy "https://purl.org/wodt/" ;
           rdfs:label "Domain tag"@en .


#################################################################
#    Object Properties
#################################################################

###  https://purl.org/wodt/dtd
:dtd rdf:type owl:ObjectProperty ;
     rdfs:comment "This property allows to link to the associated Digital Twin Description"@en ;
     rdfs:isDefinedBy "https://purl.org/wodt/" ;
     rdfs:label "Digital Twin Description"@en .


###  https://purl.org/wodt/dtkg
:dtkg rdf:type owl:ObjectProperty ;
      rdfs:comment "This property links the Digital Twin Description to its Digital Twin Knowledge Graph."@en ;
      rdfs:isDefinedBy "https://purl.org/wodt/" ;
      rdfs:label "Digital Twin Knowledge Graph"@en .


###  https://purl.org/wodt/hasDigitalTwin
:hasDigitalTwin rdf:type owl:ObjectProperty ;
                owl:inverseOf :registeredToPlatform ;
                rdfs:comment "This property links a WoDT Platform to its registered WoDT Digital Twins."@en ;
                rdfs:isDefinedBy "https://purl.org/wodt/" ;
                rdfs:label "Has registered WoDT Digital Twin"@en .


###  https://purl.org/wodt/registeredToPlatform
:registeredToPlatform rdf:type owl:ObjectProperty ;
                      rdfs:domain :WoDTDigitalTwin ;
                      rdfs:range :WoDTPlatform ;
                      rdfs:comment "This property link the WoDT Digital Twin to the WoDT Platform to which it is registered."@en ;
                      rdfs:isDefinedBy "https://purl.org/wodt/" ;
                      rdfs:label "Registered to WoDT Platform"@en .


#################################################################
#    Data properties
#################################################################

###  https://purl.org/wodt/augmentedInteraction
:augmentedInteraction rdf:type owl:DatatypeProperty ;
                      rdfs:range xsd:boolean ;
                      rdfs:comment "This property state if the interaction is an augmented one or not. If not it means that it is mirrored from the associated Physical Asset."@en ;
                      rdfs:isDefinedBy "https://purl.org/wodt/" ;
                      rdfs:label "Augmented Interaction"@en .


###  https://purl.org/wodt/availableActionId
:availableActionId rdf:type owl:DatatypeProperty ;
                   rdfs:domain :WoDTDigitalTwin ;
                   rdfs:range xsd:string ;
                   rdfs:comment "This property allows to describe the Action that are currently available on a WoDT Digital Twin."@en ;
                   rdfs:isDefinedBy "https://purl.org/wodt/" ;
                   rdfs:label "Available Action Id"@en .


###  https://purl.org/wodt/physicalAssetId
:physicalAssetId rdf:type owl:DatatypeProperty ;
                 rdfs:domain :WoDTDigitalTwin ;
                 rdfs:range xsd:string ;
                 rdfs:comment "This property indicates the Physical Asset identifier that is associated with the represented Digital Twin" ;
                 rdfs:isDefinedBy "https://purl.org/wodt/" ;
                 rdfs:label "Physical asset identifier"@en .


#################################################################
#    Classes
#################################################################

###  http://xmlns.com/foaf/0.1/Person
foaf:Person rdf:type owl:Class .


###  https://purl.org/wodt/AvailableActions
:AvailableActions rdf:type owl:Class ;
                  rdfs:subClassOf :WoDTEntity ;
                  owl:disjointWith :WoDTDigitalTwin ,
                                   :WoDTPlatform ;
                  rdfs:comment "The class that represents the WoDT Digital Twin currently available actions."@en ;
                  rdfs:isDefinedBy "https://purl.org/wodt/" ;
                  rdfs:label "Available actions"@en .


###  https://purl.org/wodt/WoDTDigitalTwin
:WoDTDigitalTwin rdf:type owl:Class ;
                 rdfs:subClassOf :WoDTEntity ;
                 owl:disjointWith :WoDTPlatform ;
                 rdfs:comment """A Digital Twin compliant with the HWoDT proposal.
Moreover, a registered WoDT Digital Twin is a WoDT Digital Twin that has added itself or has been added to a WoDT Platform.

Digital Twins refer to the ability to clone a Physical Asset (PA) through a software counterpart during its life cycle. The Digital Twin has a model that reflects all the properties, relationships, and characteristics of the physical asset that are important for the analyzed context."""@en ;
                 rdfs:isDefinedBy "https://purl.org/wodt/" ;
                 rdfs:label "WoDT Digital Twin"@en .


###  https://purl.org/wodt/WoDTEntity
:WoDTEntity rdf:type owl:Class ;
            rdfs:comment "This class includes all the classes defined under the WoDT vocabulary"@en ;
            rdfs:isDefinedBy "https://purl.org/wodt/" .


###  https://purl.org/wodt/WoDTPlatform
:WoDTPlatform rdf:type owl:Class ;
              rdfs:subClassOf :WoDTEntity ;
              rdfs:comment "A WoDT Platform is a software entity that manages the creation of the Platform Knowledge Graph by merging the data obtained from the registered WoDT Digital Twins. Based on the Platform Knowledge Graph the WoDT Platform offers services at the application level and acts as a service-layer to enable applications on top of it."@en ;
              rdfs:isDefinedBy "https://purl.org/wodt/" ;
              rdfs:label "WoDT Platform"@en .


###  Generated by the OWL API (version 4.5.26.2023-07-17T20:34:13Z) https://github.com/owlcs/owlapi
