@prefix : <https://purl.org/wodt/> .
@prefix dc: <http://purl.org/dc/elements/1.1/> .
@prefix owl: <http://www.w3.org/2002/07/owl#> .
@prefix rdf: <http://www.w3.org/1999/02/22-rdf-syntax-ns#> .
@prefix xml: <http://www.w3.org/XML/1998/namespace> .
@prefix xsd: <http://www.w3.org/2001/XMLSchema#> .
@prefix foaf: <http://xmlns.com/foaf/0.1/> .
@prefix rdfs: <http://www.w3.org/2000/01/rdf-schema#> .
@prefix time: <http://www.w3.org/2006/time#> .
@prefix vann: <http://purl.org/vocab/vann/> .
@prefix dcterms: <http://purl.org/dc/terms/> .
@base <https://purl.org/wodt/> .

<https://purl.org/wodt/> rdf:type owl:Ontology ;
                          dc:rights "This ontology is licensed under Apache 2.0" ;
                          dcterms:creator [ rdf:type foaf:Person ;
                                            foaf:name "Andrea" ;
                                            foaf:surname "Giulianelli"
                                          ] ;
                          dcterms:description "The WoDT vocabulary supports the Digital Twin Description implementation within the Hypermedia-based WoDT proposal"@en ;
                          dcterms:license <https://www.apache.org/licenses/LICENSE-2.0> ;
                          dcterms:title "WoDT vocabulary" ;
                          vann:preferredNamespacePrefix "wodt" ;
                          rdfs:label "WoDT vocabulary"@en ;
                          owl:versionInfo "1.0.0" .

#################################################################
#    Annotation properties
#################################################################

###  http://purl.org/dc/elements/1.1/rights
dc:rights rdf:type owl:AnnotationProperty .


###  http://purl.org/dc/terms/creator
dcterms:creator rdf:type owl:AnnotationProperty .


###  http://purl.org/dc/terms/description
dcterms:description rdf:type owl:AnnotationProperty .


###  http://purl.org/dc/terms/license
dcterms:license rdf:type owl:AnnotationProperty .


###  http://purl.org/dc/terms/title
dcterms:title rdf:type owl:AnnotationProperty .


###  http://purl.org/vocab/vann/preferredNamespacePrefix
vann:preferredNamespacePrefix rdf:type owl:AnnotationProperty .


###  http://xmlns.com/foaf/0.1/name
foaf:name rdf:type owl:AnnotationProperty .


###  http://xmlns.com/foaf/0.1/surname
foaf:surname rdf:type owl:AnnotationProperty .


#################################################################
#    Object Properties
#################################################################

###  https://purl.org/wodt/currentStatus
:currentStatus rdf:type owl:ObjectProperty ;
               rdfs:comment "This property links the Digital Twin Descriptor to its Digital Twin Knowledge Graph."@en ;
               rdfs:isDefinedBy "https://purl.org/wodt/" ;
               rdfs:label "Current status"@en .


###  https://purl.org/wodt/domainPredicate
:domainPredicate rdf:type owl:ObjectProperty ;
                 rdfs:range rdf:Property ;
                 rdfs:comment "This property allows to associate an element of the meta-model of the Digital Twin Descriptor to the domain."@en ;
                 rdfs:isDefinedBy "https://purl.org/wodt/" ;
                 rdfs:label "Domain predicate"@en .


###  https://purl.org/wodt/hasDescriptor
:hasDescriptor rdf:type owl:ObjectProperty ;
               rdfs:comment "This property allows to link to the associated Digital Twin Descriptor"@en ;
               rdfs:isDefinedBy "https://purl.org/wodt/" ;
               rdfs:label "Has Digital Twin Descriptor"@en .


###  https://purl.org/wodt/hasDigitalTwin
:hasDigitalTwin rdf:type owl:ObjectProperty ;
                owl:inverseOf :registeredToPlatform ;
                rdfs:comment "This property links a WoDT Digital Twins Platform to its registered WoDT Digital Twins."@en ;
                rdfs:isDefinedBy "https://purl.org/wodt/" ;
                rdfs:label "Has registered WoDT Digital Twin"@en .


###  https://purl.org/wodt/registeredToPlatform
:registeredToPlatform rdf:type owl:ObjectProperty ;
                      rdfs:domain :WoDTDigitalTwin ;
                      rdfs:range :WoDTPlatform ;
                      rdfs:comment "This property link the WoDT Digital Twin to the WoDT Digital Twins Platform to which it is registered."@en ;
                      rdfs:isDefinedBy "https://purl.org/wodt/" ;
                      rdfs:label "Registered to WoDT Digital Twins Platform"@en .


###  https://purl.org/wodt/shadowingLatency
:shadowingLatency rdf:type owl:ObjectProperty ,
                           owl:FunctionalProperty ;
                  rdfs:domain :WoDTDigitalTwin ;
                  rdfs:range time:Duration ;
                  rdfs:comment "This property represents the shadowing latency of the Digital Twin"@en ;
                  rdfs:isDefinedBy "https://purl.org/wodt/" ;
                  rdfs:label "Shadowing latency"@en .


#################################################################
#    Data properties
#################################################################

###  https://purl.org/wodt/actionId
:actionId rdf:type owl:DatatypeProperty ;
          rdfs:range xsd:string ;
          rdfs:comment "This property allows to link an Action affordance to its Action identifier."@en ;
          rdfs:isDefinedBy "https://purl.org/wodt/" ;
          rdfs:label "Action Id"@en .


###  https://purl.org/wodt/augmentedInteraction
:augmentedInteraction rdf:type owl:DatatypeProperty ;
                      rdfs:range xsd:boolean ;
                      rdfs:comment "This property state if the interaction is an augmented one or not. If not it means that it is mirrored from the associated Physical Asset."@en ;
                      rdfs:isDefinedBy "https://purl.org/wodt/" ;
                      rdfs:label "Augmented Interaction"@en .


###  https://purl.org/wodt/availableActionId
:availableActionId rdf:type owl:DatatypeProperty ;
                   rdfs:domain :WoDTDigitalTwin ;
                   rdfs:range xsd:string ;
                   rdfs:comment "This property allows to describe the Action that are currently available on a WoDT Digital Twin."@en ;
                   rdfs:isDefinedBy "https://purl.org/wodt/" ;
                   rdfs:label "Available Action Id"@en .


###  https://purl.org/wodt/deploymentCountry
:deploymentCountry rdf:type owl:DatatypeProperty ;
                   rdfs:domain :WoDTDigitalTwin ;
                   rdfs:range xsd:string ;
                   rdfs:comment "The deployment country of the Digital Twin. The country is expressed following the ISO 3166-1 alpha-2 or alpha-3 country codes."@en ;
                   rdfs:isDefinedBy "https://purl.org/wodt/" ;
                   rdfs:label "Deployment country"@en .


###  https://purl.org/wodt/physicalAssetId
:physicalAssetId rdf:type owl:DatatypeProperty ;
                 rdfs:domain :WoDTDigitalTwin ;
                 rdfs:range xsd:string ;
                 rdfs:comment "This property indicates the Physical Asset identifier that is associated with the represented Digital Twin" ;
                 rdfs:isDefinedBy "https://purl.org/wodt/" ;
                 rdfs:label "Physical asset identifier"@en .


###  https://purl.org/wodt/propertyTolerance
:propertyTolerance rdf:type owl:DatatypeProperty ;
                   rdfs:range xsd:double ;
                   rdfs:comment "This property represents the tolerance of the described property. The unit of measurement is the same of the associated property."@en ;
                   rdfs:isDefinedBy "https://purl.org/wodt/" ;
                   rdfs:label "Property tolerance"@en .


###  https://purl.org/wodt/version
:version rdf:type owl:DatatypeProperty ;
         rdfs:domain :WoDTDigitalTwin ;
         rdfs:range xsd:string ;
         rdfs:comment "This property describes the version of the Digital Twin Descriptor"@en ;
         rdfs:isDefinedBy "https://purl.org/wodt/" ;
         rdfs:label "Version"@en .


#################################################################
#    Classes
#################################################################

###  http://www.w3.org/1999/02/22-rdf-syntax-ns#Property
rdf:Property rdf:type owl:Class .


###  http://www.w3.org/2006/time#Duration
time:Duration rdf:type owl:Class .


###  http://www.w3.org/2006/time#TemporalUnit
time:TemporalUnit rdf:type owl:Class .


###  http://xmlns.com/foaf/0.1/Person
foaf:Person rdf:type owl:Class .


###  https://purl.org/wodt/WoDTDigitalTwin
:WoDTDigitalTwin rdf:type owl:Class ;
                 rdfs:subClassOf :WoDTEntity ;
                 rdfs:comment """A Digital Twin compliant with the HWoDT proposal.
Moreover, a registered WoDT Digital Twin is a WoDT Digital Twin that has added itself or has been added to a WoDT Platform.

Digital Twins refer to the ability to clone a Physical Asset (PA) through a software counterpart during its life cycle. The Digital Twin has a model that reflects all the properties, relationships, and characteristics of the physical asset that are important for the analyzed context."""@en ;
                 rdfs:isDefinedBy "https://purl.org/wodt/" ;
                 rdfs:label "WoDT Digital Twin"@en .


###  https://purl.org/wodt/WoDTEntity
:WoDTEntity rdf:type owl:Class ;
            rdfs:comment "This class includes all the classes defined under the WoDT vocabulary"@en ;
            rdfs:isDefinedBy "https://purl.org/wodt/" .


###  https://purl.org/wodt/WoDTPlatform
:WoDTPlatform rdf:type owl:Class ;
              rdfs:subClassOf :WoDTEntity ;
              rdfs:comment "A WoDT Platform is a software entity that manages the creation of the Platform Knowledge Graph by merging the data obtained from the registered WoDT Digital Twins. Based on the Platform Knowledge Graph the WoDT Platform offers services at the application level and acts as a service-layer to enable applications on top of it."@en ;
              rdfs:isDefinedBy "https://purl.org/wodt/" ;
              rdfs:label "WoDT Platform"@en .


#################################################################
#    Individuals
#################################################################

###  https://purl.org/wodt/unitMillisecond
:unitMillisecond rdf:type owl:NamedIndividual ,
                          time:TemporalUnit ;
                 rdfs:comment "The TemporalUnit instance that represents milliseconds."@en ;
                 rdfs:isDefinedBy "https://purl.org/wodt/" ;
                 rdfs:label "Milliseconds unit of measurement"@en .


###  Generated by the OWL API (version 4.5.26.2023-07-17T20:34:13Z) https://github.com/owlcs/owlapi
